NoInit.v
@@ -7,6 +7,12 @@ From Elo Require Import Core.
 Inductive no_init (ad : addr) : tm -> Prop :=
   | noinit_unit  :                  no_init ad <{unit                     }>
   | noinit_nat   : forall n,        no_init ad <{nat n                    }>
+  | noinit_plus  : forall t1 t2,    no_init ad t1 ->
+                                    no_init ad t2 ->
+                                    no_init ad <{t1 + t2                  }>
+  | noinit_monus : forall t1 t2,    no_init ad t1 ->
+                                    no_init ad t2 ->
+                                    no_init ad <{t1 - t2                  }>
   | noinit_seq   : forall t1 t2,    no_init ad t1 ->
                                     no_init ad t2 ->
                                     no_init ad <{t1; t2                   }>
@@ -49,6 +55,8 @@ Local Ltac _noinit tt :=
   match goal with
   | H : no_init _   <{unit                  }> |- _ => clear H
   | H : no_init _   <{nat _                 }> |- _ => clear H
+  | H : no_init _   <{_ + _                 }> |- _ => tt H
+  | H : no_init _   <{_ - _                 }> |- _ => tt H
   | H : no_init _   <{_; _                  }> |- _ => tt H
   | H : no_init _   <{if _ then _ else _ end}> |- _ => tt H
   | H : no_init _   <{while _ do _ end      }> |- _ => tt H
@@ -197,6 +205,14 @@ Definition no_inits (t : tm) := forall ad, no_init ad t.
 Local Ltac solve_inv_noinits :=
   unfold no_inits; intros; repeat split; intros; spec; invc_noinit; auto.
 
+Local Lemma inv_noinits_plus : forall t1 t2,
+  no_inits <{t1 + t2}> -> no_inits t1 /\ no_inits t2.
+Proof. solve_inv_noinits. Qed.
+
+Local Lemma inv_noinits_monus : forall t1 t2,
+  no_inits <{t1 - t2}> -> no_inits t1 /\ no_inits t2.
+Proof. solve_inv_noinits. Qed.
+
 Local Lemma inv_noinits_seq : forall t1 t2,
   no_inits <{t1; t2}> -> no_inits t1 /\ no_inits t2.
 Proof. solve_inv_noinits. Qed.
@@ -249,6 +265,8 @@ Ltac invc_noinits :=
 match goal with
 | H : no_inits <{unit        }> |- _ => clear H
 | H : no_inits <{nat _       }> |- _ => clear H
+| H : no_inits <{_ + _       }> |- _ => eapply inv_noinits_plus  in H as [? ?]
+| H : no_inits <{_ - _       }> |- _ => eapply inv_noinits_monus in H as [? ?]
 | H : no_inits <{_; _        }> |- _ => eapply inv_noinits_seq in H as [? ?]
 | H : no_inits (tm_if _ _ _  )  |- _ => eapply inv_noinits_if  in H as [? [? ?]]
 | H : no_inits (tm_while _ _ )  |- _ => eapply inv_noinits_while in H as [? ?]
